WPDS/FinFunWeakSaturation.thy
@@ -1,0 +1,352 @@
+theory FinFunWeakSaturation
+  imports "Saturation" "FinFunAddUpdate"
+begin
+
+
+inductive non_equal_rule :: "'t saturation_rule \<Rightarrow> 't saturation_rule" for rule where
+  rule_to_non_equal_rule: "rule ts ts' \<Longrightarrow> ts \<noteq> ts' \<Longrightarrow> non_equal_rule rule ts ts'"
+
+inductive weak_rule :: "'t::idempotent_ab_semigroup_add_ord saturation_rule \<Rightarrow> 't saturation_rule" for rule where
+  rule_to_weak_rule: "rule ts ts'' \<Longrightarrow> ts'' \<le> ts' \<Longrightarrow> ts' < ts \<Longrightarrow> weak_rule rule ts ts'"
+
+locale rule_saturation =
+  fixes rule :: "'t::idempotent_ab_semigroup_add_ord saturation_rule"
+  assumes rule_less_eq: "rule ts ts' \<Longrightarrow> ts' \<le> ts"
+  assumes rule_mono: "ts\<^sub>3 \<le> ts\<^sub>1 \<Longrightarrow> rule ts\<^sub>1 ts\<^sub>2 \<Longrightarrow> \<exists>ts'. rule ts\<^sub>3 ts' \<and> ts' \<le> ts\<^sub>2"
+begin
+
+lemma rule_exists_addition: "rule ts ts' \<Longrightarrow> \<exists>a. ts' = ts + a"
+  using order_prop rule_less_eq add.commute by metis
+lemma weak_rule_exists_addition: "weak_rule rule a b \<Longrightarrow> \<exists>c. b = a + c"
+  unfolding weak_rule.simps by (metis meet.inf.absorb4) 
+
+lemma rule_add_extend: 
+  assumes "rule ts\<^sub>1 ts\<^sub>2"
+  shows "\<exists>ts'. rule (ts + ts\<^sub>1) (ts + ts') \<and> ts' \<le> ts\<^sub>2"
+proof -
+  obtain ts' where ts': "rule (ts + ts\<^sub>1) ts'" "ts' \<le> ts\<^sub>2"
+    using rule_mono[of "ts + ts\<^sub>1" ts\<^sub>1 ts\<^sub>2] assms by auto
+  then have "rule (ts + ts\<^sub>1) (ts + ts')" 
+    using rule_less_eq[OF ts'(1)] meet.inf.absorb2 by fastforce
+  then show ?thesis using ts'(2) by blast
+qed
+
+lemma non_equal_rule_less: "non_equal_rule rule a b \<Longrightarrow> b < a"
+  using rule_less_eq by (metis non_equal_rule.simps order_le_imp_less_or_eq)
+lemma non_equal_rule_less_eq: "non_equal_rule rule a b \<Longrightarrow> b \<le> a"
+  using non_equal_rule_less by fastforce
+
+lemma weak_rule_less: "weak_rule rule ts ts' \<Longrightarrow> ts' < ts"
+  using weak_rule.simps by blast
+lemma weak_rule_less_eq: "weak_rule rule ts ts' \<Longrightarrow> ts' \<le> ts"
+  using weak_rule_less  by fastforce
+
+lemma weak_rule_star_less_eq: "(weak_rule rule)\<^sup>*\<^sup>* ts ts' \<Longrightarrow> ts' \<le> ts"
+  apply (induct rule: rtranclp_induct, simp)
+  using weak_rule_less_eq by fastforce
+
+lemma weak_rule_intro: "non_equal_rule rule ts ts' \<Longrightarrow> weak_rule rule ts ts'"
+  using rule_to_weak_rule[of rule ts ts'] non_equal_rule.cases[of rule ts ts'] order_refl
+  by (metis non_equal_rule_less)
+
+lemma weak_rule_star_intro: "(non_equal_rule rule)\<^sup>*\<^sup>* ts ts' \<Longrightarrow> (weak_rule rule)\<^sup>*\<^sup>* ts ts'"
+  apply(induct rule: rtranclp_induct, simp)
+  using weak_rule_intro by fastforce
+
+lemma weak_rule_star_to_non_equal_rule_star:
+  assumes "(weak_rule rule)\<^sup>*\<^sup>* ts ts'"
+  shows "\<exists>ts''. (non_equal_rule rule)\<^sup>*\<^sup>* ts ts'' \<and> ts'' \<le> ts'"
+  using assms
+proof (induction rule: rtranclp_induct)
+  case base
+  then show ?case by blast
+next
+  case (step ts\<^sub>1 ts\<^sub>2)
+  obtain ts'' where ts'': "rule ts\<^sub>1 ts''" "ts'' \<le> ts\<^sub>2"
+    using step(2) weak_rule.simps by blast
+  obtain ts\<^sub>3 where ts3: "(non_equal_rule rule)\<^sup>*\<^sup>* ts ts\<^sub>3" "ts\<^sub>3 \<le> ts\<^sub>1"
+    using step(3) by blast
+  obtain ts\<^sub>4 where ts4: "rule ts\<^sub>3 ts\<^sub>4" "ts\<^sub>4 \<le> ts''"
+    using rule_mono[of ts\<^sub>3 ts\<^sub>1 ts''] ts3(2) ts''(1) by fast
+  have "ts\<^sub>4 \<le> ts\<^sub>2" using ts4(2) ts''(2) by fastforce
+  show ?case
+  proof (cases "ts\<^sub>3 = ts\<^sub>4")
+    case True
+    then show ?thesis using \<open>ts\<^sub>4 \<le> ts\<^sub>2\<close> ts3(1) by blast
+  next
+    case False
+    then have "non_equal_rule rule ts\<^sub>3 ts\<^sub>4"
+      using ts4(1) non_equal_rule.intros by metis
+    then show ?thesis using \<open>ts\<^sub>4 \<le> ts\<^sub>2\<close> rtranclp.rtrancl_into_rtrancl[OF ts3(1)]
+      by blast
+  qed
+qed
+
+
+lemma weak_rule_step_mono:
+  assumes "ts\<^sub>2 \<le> ts\<^sub>1"
+  assumes "weak_rule rule ts\<^sub>1 ts\<^sub>3"
+  shows "(weak_rule rule)\<^sup>*\<^sup>* ts\<^sub>2 (ts\<^sub>2 + ts\<^sub>3)"
+proof -
+  obtain a\<^sub>3 where ts3: "ts\<^sub>3 = ts\<^sub>1 + a\<^sub>3" 
+    using weak_rule_exists_addition[OF assms(2)] by fast
+  obtain ts' where ts': "rule ts\<^sub>1 ts'" "ts' \<le> ts\<^sub>3"
+    using assms(2) weak_rule.simps by blast
+  obtain ts\<^sub>4 where ts4: "rule ts\<^sub>2 ts\<^sub>4" "ts\<^sub>4 \<le> ts'"
+    using rule_mono assms(1) ts'(1) by blast
+  have eq: "ts\<^sub>2 + a\<^sub>3 = ts\<^sub>2 + ts\<^sub>3" unfolding ts3
+    using assms(1)[unfolded less_eq_def, symmetric] by (metis meet.inf_assoc)
+  show ?thesis proof (cases "ts\<^sub>2 = ts\<^sub>2 + a\<^sub>3")
+    case True
+    then show ?thesis using eq unfolding ts3 by simp
+  next
+    case False
+    then have le:"ts\<^sub>2 + a\<^sub>3 < ts\<^sub>2" by (simp add: order_le_neq_trans)
+    have "weak_rule rule ts\<^sub>2 (ts\<^sub>2 + a\<^sub>3)"
+      using weak_rule.intros[of rule, OF ts4(1) _ le]
+            ts4(2) ts'(2)[unfolded ts3] rule_less_eq[OF ts4(1)] 
+      by fastforce
+    then show ?thesis using eq unfolding ts3 by auto
+  qed
+qed
+
+lemma weak_rule_step_mono':
+  assumes "(weak_rule rule)\<^sup>*\<^sup>* ts\<^sub>1 ts\<^sub>2"
+  assumes "weak_rule rule ts\<^sub>1 ts\<^sub>3"
+  shows "(weak_rule rule)\<^sup>*\<^sup>* ts\<^sub>1 (ts\<^sub>2 + ts\<^sub>3)"
+  using rtranclp_trans[of "weak_rule rule" ts\<^sub>1 ts\<^sub>2 "ts\<^sub>2 + ts\<^sub>3", OF assms(1)]
+  using assms(2) weak_rule_star_less_eq[OF assms(1)] weak_rule_step_mono by simp
+
+lemma weak_rule_add_extend:
+  assumes "weak_rule rule ts\<^sub>1 ts\<^sub>2"
+  assumes "ts + ts\<^sub>1 \<noteq> ts + ts\<^sub>2"
+  shows "weak_rule rule (ts + ts\<^sub>1) (ts + ts\<^sub>2)"
+proof -
+  obtain ts' where ts': "rule ts\<^sub>1 ts'" "ts' \<le> ts\<^sub>2" (*"ts\<^sub>1 \<noteq> ts\<^sub>2"*)
+    by (metis assms(1) weak_rule.simps)
+  obtain ts'' where ts'': "rule (ts + ts\<^sub>1) (ts + ts'')" "ts'' \<le> ts'"
+    using ts'(1) rule_add_extend by blast
+  have "ts + ts\<^sub>2 < ts + ts\<^sub>1" using assms(2) weak_rule_less[OF assms(1)]
+    by (simp add: meet.inf.strict_order_iff meet.inf_commute meet.inf_left_commute)
+  then show ?thesis                                                                                                  
+    using rule_to_weak_rule[of rule "ts + ts\<^sub>1" "ts + ts''" "ts + ts\<^sub>2", OF ts''(1)]
+    using order.trans[OF ts''(2) ts'(2)] meet.inf_mono by blast
+qed
+
+lemma weak_rule_add_mono:
+  assumes "(weak_rule rule)\<^sup>*\<^sup>* ts (ts + ts\<^sub>1)"
+  assumes "(weak_rule rule) ts\<^sub>1 ts\<^sub>2"
+  shows "(weak_rule rule)\<^sup>*\<^sup>* ts (ts + ts\<^sub>2)"
+proof (cases "ts + ts\<^sub>1 = ts + ts\<^sub>2")
+  case True
+  then show ?thesis using assms(1) by simp
+next
+  case False
+  then have "(weak_rule rule) (ts + ts\<^sub>1) (ts + ts\<^sub>2)" 
+    using assms(2) weak_rule_add_extend by blast
+  then show ?thesis using assms(1) by simp
+qed
+
+lemma weak_rule_add_star_mono:
+  assumes "(weak_rule rule)\<^sup>*\<^sup>* ts\<^sub>1 ts\<^sub>2"
+  assumes "(weak_rule rule)\<^sup>*\<^sup>* ts (ts + ts\<^sub>1)"
+  shows "(weak_rule rule)\<^sup>*\<^sup>* ts (ts + ts\<^sub>2)"
+  using assms(1,2)
+  by (induct rule: rtranclp_induct, simp_all add: weak_rule_add_mono)
+
+
+lemma weak_rule_star_mono:
+  assumes "(weak_rule rule)\<^sup>*\<^sup>* ts\<^sub>1 ts\<^sub>2"
+  assumes "(weak_rule rule)\<^sup>*\<^sup>* ts\<^sub>1 ts\<^sub>3"
+  shows "(weak_rule rule)\<^sup>*\<^sup>* ts\<^sub>2 (ts\<^sub>2 + ts\<^sub>3)"
+    using assms(2,1)
+proof (induction rule: converse_rtranclp_induct)
+  case base
+  then show ?case by (metis meet.inf.orderE weak_rule_star_less_eq rtranclp.simps)
+next
+  case (step ts\<^sub>1' ts\<^sub>3')
+  show ?case using weak_rule_add_star_mono[OF step(2) weak_rule_step_mono[OF weak_rule_star_less_eq[OF step(4)] step(1)]] 
+    by blast
+qed
+
+lemma saturated_non_equal_to_weak:
+  "saturated (non_equal_rule rule) ts \<Longrightarrow> saturated (weak_rule rule) ts"
+  unfolding saturated_def non_equal_rule.simps weak_rule.simps by force
+lemma saturated_weak_to_non_equal:
+  "saturated (weak_rule rule) ts \<Longrightarrow> saturated (non_equal_rule rule) ts"
+  unfolding saturated_def non_equal_rule.simps weak_rule.simps 
+  by (meson dual_order.order_iff_strict rule_less_eq)
+
+lemma saturated_weak_rule_star_less_eq:
+  assumes "(weak_rule rule)\<^sup>*\<^sup>* ts\<^sub>1 ts\<^sub>2"
+  assumes "(weak_rule rule)\<^sup>*\<^sup>* ts\<^sub>1 ts\<^sub>3"
+  assumes "saturated (weak_rule rule) ts\<^sub>3"
+  shows "ts\<^sub>3 \<le> ts\<^sub>2"
+  using weak_rule_star_mono[OF assms(2,1)] assms(3)[unfolded saturated_def]
+  unfolding idempotent_ab_semigroup_add_ord_class.less_eq_def
+  using converse_rtranclpE[of "weak_rule rule" ts\<^sub>3 "ts\<^sub>3 + ts\<^sub>2"] by metis
+
+context 
+  fixes rule'
+  assumes weak_star_intro: "(non_equal_rule rule')\<^sup>*\<^sup>* ts ts' \<Longrightarrow> (weak_rule rule)\<^sup>*\<^sup>* ts ts'"
+  assumes preserves_saturated: "saturated (non_equal_rule rule') ts \<Longrightarrow> saturated (non_equal_rule rule) ts"
+begin
+
+lemma preserves_saturation:
+  assumes "saturation (non_equal_rule rule') ts ts'"
+  shows "saturation (non_equal_rule rule) ts ts'"
+proof -
+  have star':"(non_equal_rule rule')\<^sup>*\<^sup>* ts ts'" using assms unfolding saturation_def by argo
+  have sat:"saturated (weak_rule rule) ts'" 
+    using assms unfolding saturation_def using preserves_saturated[THEN saturated_non_equal_to_weak] by simp
+  have weak:"(weak_rule rule)\<^sup>*\<^sup>* ts ts'" using weak_star_intro[OF star'] by fast
+  obtain ts\<^sub>3 where rule:"(non_equal_rule rule)\<^sup>*\<^sup>* ts ts\<^sub>3" and leq:"ts\<^sub>3 \<le> ts'" 
+    using weak_rule_star_to_non_equal_rule_star[OF weak] by blast
+  have "ts' \<le> ts\<^sub>3" using saturated_weak_rule_star_less_eq[OF weak_rule_star_intro[OF rule] weak sat] by simp
+  then have "ts' = ts\<^sub>3" using leq by auto                                                     
+  then have "(non_equal_rule rule)\<^sup>*\<^sup>* ts ts'" using rule by fast
+  then show ?thesis using assms preserves_saturated unfolding saturation_def by simp
+qed
+
+end
+
+lemma saturation_non_equal_is_weak:
+  "saturation (non_equal_rule rule) ts ts' \<longleftrightarrow> saturation (weak_rule rule) ts ts'"
+proof
+  show "saturation (non_equal_rule rule) ts ts' \<Longrightarrow> saturation (weak_rule rule) ts ts'"
+    unfolding saturation_def using saturated_non_equal_to_weak weak_rule_star_intro by auto
+  assume assm: "saturation (weak_rule rule) ts ts'"
+  have star:"(weak_rule rule)\<^sup>*\<^sup>* ts ts'" using assm unfolding saturation_def by argo
+  have satW:"saturated (weak_rule rule) ts'" using assm unfolding saturation_def by blast
+  then have sat:"saturated (non_equal_rule rule) ts'" using saturated_weak_to_non_equal by blast
+  obtain ts'' where ts'': "(non_equal_rule rule)\<^sup>*\<^sup>* ts ts''" "ts'' \<le> ts'"
+    using weak_rule_star_to_non_equal_rule_star[OF star] by blast
+  then show "saturation (non_equal_rule rule) ts ts'" unfolding saturation_def using sat
+    using saturated_weak_rule_star_less_eq[OF weak_rule_star_intro[OF ts''(1)] star satW] by simp
+qed
+
+end
+
+
+locale step_saturation = 
+  fixes step::"('a::finite \<Rightarrow>f 'b::bounded_idempotent_semiring) \<Rightarrow> ('a::finite \<Rightarrow>f 'b::bounded_idempotent_semiring)"
+begin
+  definition "step_loop = while_option (\<lambda>s. step s \<noteq> s) (step)"
+  definition "step_exec = the o step_loop"
+  definition "step_rule ts ts' \<equiv> step ts = ts'"
+end
+locale decreasing_step_saturation = step_saturation step
+  for step::"('a::finite \<Rightarrow>f 'b::bounded_idempotent_semiring) \<Rightarrow> ('a::finite \<Rightarrow>f 'b::bounded_idempotent_semiring)" +
+(*  assumes weak_rule_star_step: "(weak_rule rule)\<^sup>*\<^sup>* S (step S)"*)
+  assumes step_decreasing: "step S \<le> S"
+(*  assumes step_fixpoint_is_rule_saturated: "step t = t \<Longrightarrow> \<forall>ts. \<not> (weak_rule rule) t ts"*)
+begin
+
+lemma step_exec_terminates: 
+  shows "\<exists>t. step_loop S = Some t"
+  unfolding step_loop_def 
+  using wf_rel_while_option_Some[OF wf_less_finfun, of "\<lambda>S. step S \<le> S" "(\<lambda>S. step S \<noteq> S)" step S]
+        step_decreasing
+  by fastforce
+
+lemma step_rule_star_step: "(non_equal_rule step_rule)\<^sup>*\<^sup>* S (step S)"
+  unfolding step_rule_def non_equal_rule.simps by (cases "S = step S") auto
+lemma weak_rule_star_step_k: "(non_equal_rule step_rule)\<^sup>*\<^sup>* S ((step ^^ k) S)"
+  by (induct k) (auto elim!: rtranclp_trans intro: step_rule_star_step)
+
+lemma saturation_step_exec': "saturation (non_equal_rule step_rule) S (step_exec S)"
+proof -
+  from step_exec_terminates obtain t where t: "step_loop S = Some t" by blast
+  obtain k where k: "t = (step ^^ k) S" and eq: "step t = t"
+    using while_option_stop2[OF t[unfolded step_loop_def]] by auto
+  have "\<And>ts. \<not> (non_equal_rule step_rule) t ts" 
+    using eq unfolding non_equal_rule.simps step_rule_def by presburger
+  then show ?thesis
+    unfolding saturation_def saturated_def step_exec_def o_apply t
+    by (simp_all add: weak_rule_star_step_k k)
+qed
+
+end
+
+locale sum_saturation = decreasing_step_saturation step + rule_saturation rule
+  for step::"('a::finite \<Rightarrow>f 'b::bounded_idempotent_semiring) \<Rightarrow> ('a::finite \<Rightarrow>f 'b::bounded_idempotent_semiring)"
+  and rule :: "('a::finite \<Rightarrow>f 'b::bounded_idempotent_semiring) saturation_rule" +
+  assumes step_is_sum: "step ts = ts + \<Sum>{ts'. non_equal_rule rule ts ts'}"
+  assumes finite_rule_set: "finite {ts'. non_equal_rule rule ts ts'}"
+begin
+
+lemma non_equal_rule_step_not_fixp:
+  assumes "non_equal_rule rule ts ts'"
+  shows "ts + \<Sum> {ts'. non_equal_rule rule ts ts'} \<noteq> ts"
+proof (cases "{ts'. non_equal_rule rule ts ts'} = {}")
+  case True
+  then show ?thesis using assms by blast
+next
+  case False
+  have le:"\<Sum> {ts'. non_equal_rule rule ts ts'} \<le> ts" 
+    using sum_smaller_elem[of "{ts'. non_equal_rule rule ts ts'}" ts, OF _ finite_rule_set False] non_equal_rule_less_eq 
+    by blast
+  have le':"\<Sum> {ts'. non_equal_rule rule ts ts'} \<le> ts'"
+    unfolding BoundedDioid.idempotent_ab_semigroup_add_ord_class.less_eq_def 
+    using idem_sum_elem[OF finite_rule_set, of ts'] assms 
+    by (simp add: add.commute)
+  obtain a where "ts' = ts + a" and "ts' \<noteq> ts"
+    using assms unfolding non_equal_rule.simps[of rule] 
+    using non_equal_rule_less_eq[OF assms] order_prop[of ts' ts] add.commute
+    by metis
+  then have "ts + ts' \<noteq> ts" by simp
+  then show ?thesis 
+    using le le' unfolding less_eq_def using add.commute
+    by metis
+qed
+
+lemma step_fixp_implies_rule_fixp: 
+  assumes "step ts = ts"
+  assumes "rule ts ts'"
+  shows "ts = ts'" 
+proof -
+  have "Collect (non_equal_rule rule ts) = {}" 
+    using assms(1) unfolding step_is_sum using non_equal_rule_step_not_fixp
+    by fast
+  then show ?thesis using assms(2) 
+    unfolding non_equal_rule.simps by simp
+qed
+
+lemma weak_star_step: "(weak_rule rule)\<^sup>*\<^sup>* ts (step ts)"
+proof -
+  {
+    fix X
+    assume "finite X" and "X \<subseteq> {ts'. non_equal_rule rule ts ts'}"
+    then have "(weak_rule rule)\<^sup>*\<^sup>* ts (ts + \<Sum>X)"
+    proof (induct rule: finite_induct)
+      case empty
+      then show ?case by simp
+    next
+      case (insert x F)
+      then have A:"(weak_rule rule)\<^sup>*\<^sup>* ts (ts + \<Sum> F)" and B: "(non_equal_rule rule) ts x" by auto
+      have "(weak_rule rule)\<^sup>*\<^sup>* ts (ts + \<Sum> F + x)"
+        using weak_rule_step_mono'[OF A weak_rule_intro[OF B]] by blast
+      then show ?case
+        by (simp add: insert.hyps(1) meet.inf_commute meet.inf_left_commute)
+    qed
+  } 
+  then show ?thesis unfolding step_is_sum using finite_rule_set by blast
+qed
+
+lemma weak_star_intro: "(non_equal_rule step_rule)\<^sup>*\<^sup>* ts ts' \<Longrightarrow> (weak_rule rule)\<^sup>*\<^sup>* ts ts'"
+  apply (induct rule: rtranclp_induct, simp)
+  unfolding step_rule_def non_equal_rule.simps using weak_star_step rtranclp_trans 
+  by metis
+
+lemma preserves_saturated: "saturated (non_equal_rule step_rule) ts \<Longrightarrow> saturated (non_equal_rule rule) ts"
+  unfolding saturated_def step_rule_def non_equal_rule.simps using step_fixp_implies_rule_fixp by presburger
+
+lemma saturation_step_exec: "saturation (non_equal_rule rule) S (step_exec S)"
+  using rule_saturation.preserves_saturation[unfolded rule_saturation_def, of rule step_rule]
+        rule_less_eq rule_mono weak_star_intro preserves_saturated saturation_step_exec'
+  by auto
+
+end
+
+
+end
